coq/Progress.v
@@ -9,35 +9,17 @@ red_spec_object_define_own_prop_5_generic
 
 ==> get rid of the events in pretty rules (with a flag)
 
-
 ====================
-
-Arthur:
+Waiting for fixes:
 
 red_spec_object_put_3_not_data 
 red_spec_object_put_4_accessor 
 red_spec_object_put_4_not_accessor_object 
 red_spec_object_put_4_not_accessor_prim 
 
-red_spec_object_get_1_function 
-red_spec_function_get_1_error 
-red_spec_function_get_1_normal 
-red_spec_object_has_instance 
-red_spec_object_has_instance_1_prim 
-red_spec_object_has_instance_1_object 
-red_spec_function_has_instance_1_prim 
-red_spec_function_has_instance_1_object 
+====================
 
-
-red_spec_creating_function_object_proto 
-red_spec_creating_function_object_proto_1 
-red_spec_creating_function_object_proto_2 
-red_spec_creating_function_object 
-red_spec_creating_function_object_1 
-red_spec_creating_function_object_2_not_strict 
-red_spec_creating_function_object_2_strict 
-red_spec_creating_function_object_3 
-red_spec_creating_function_object_4 
+Arthur:
 
 red_spec_to_descriptor_not_object 
 red_spec_to_descriptor_object 
@@ -69,36 +51,6 @@ red_spec_to_descriptor_6c_error
 red_spec_to_descriptor_6c_ok 
 red_spec_to_descriptor_7_error 
 red_spec_to_descriptor_7_ok 
-
-red_spec_create_new_function_in 
-
-red_javascript_intro 
-(* Need a more precise lemma for [spec_binding_inst], and I need that someone reread the comments I've put in the rule [red_javascript_intro]. *)
-
-red_spec_convert_twice 
-red_spec_convert_twice_1 
-red_spec_convert_twice_2 
-red_spec_to_int32 
-red_spec_to_int32_1 
-red_spec_to_uint32 
-red_spec_to_uint32_1 
-
-switch
-do_while
-binary ops
-
-====================
-
-Martin:
-
-new program for prog_block
-
-new program for do_while
-
-
-Implementing the new stat_block, and code do_while, following while.
-
-Merging if_success* (in a branch)
 
 
 red_spec_call 
@@ -146,6 +98,39 @@ red_spec_call_global_eval_2
 red_spec_call_global_eval_3_normal_value 
 red_spec_call_global_eval_3_normal_empty 
 red_spec_call_global_eval_3_throw 
+
+
+red_spec_create_new_function_in 
+
+red_javascript_intro 
+(* Need a more precise lemma for [spec_binding_inst], and I need that someone reread the comments I've put in the rule [red_javascript_intro]. *)
+
+red_spec_convert_twice 
+red_spec_convert_twice_1 
+red_spec_convert_twice_2 
+red_spec_to_int32 
+red_spec_to_int32_1 
+red_spec_to_uint32 
+red_spec_to_uint32_1 
+
+switch
+do_while
+binary ops
+
+====================
+
+Martin:
+
+new program for prog_block
+
+new program for do_while
+
+
+Implementing the new stat_block, and code do_while, following while.
+
+Merging if_success* (in a branch)
+
+
 
 red_spec_entering_eval_code 
 red_spec_entering_eval_code_1 
@@ -260,32 +245,3 @@ red_spec_object_delete_args_obj_4
 
 
 
-
-
-
-
-
-==============================================
-
-*) Say that we formalize all of the core language (out of libraries).
-   About JS-specific functions from library: 
-   work in progress (almost all specified, no jscert-to-jsref proof yet)
-
-*) Section 4:
--- count the number pages of ES5 that we actually cover
-
-*) Section 6:
-Section 6 needs to be filled (without using too much space)
--- section 6.1: not sure it brings new information compared with what's been said before
-
-*) Section 5: 
--- Figure 7 contains "Fixpoint build_runs max_step" which is redundant with the previous def
--- Figure 4 needs to inline the definition of "vret", which is not defined
--- There is undefined reference to "abort"; 
--- An example what how the abort rule propagates exceptions (we don't have to show the generic abort rule though, we can just say that all abort rules are actually factorized as one, see pretty-big-step paper for details).
-
-*) running spellchecker on paper
-
-*) try to see if \paragraph would look nicer than \stitle
-
-*) to release Coq scripts, we'll need a script for hiding LATER and TODO (using a regexp)
